\documentclass{article}
\usepackage[fleqn]{amsmath}
\usepackage{physics}
\usepackage{mathrsfs}
\usepackage{amssymb}
\usepackage{microtype}
\newcommand{\RN}[1]{%s
  \textup{\uppercase\expandafter{\romannumeral#1}}%
}
\usepackage{geometry}
\geometry{
 a4paper,
 left=20mm,
 right=20mm,
 top=15mm,
 bottom=20mm
 }
\begin{document}
Equation of motion in Heisenberg picture with Quadratic Hamiltonian.\\
let $\hbar$ = 1.
\begin{flalign*}
    \frac{\partial}{\partial t} a_\nu = -i[H,a_\nu]
\end{flalign*}
Where H represents the Hamiltonian
\begin{flalign*}
    [ \sum_{\nu\nu'} \epsilon_{\nu\nu'} a_\nu a^\dagger_{\nu'} , a_{\nu} ] 
    &= \sum_{\nu\nu'} \epsilon_{\nu\nu'}a_\nu a^\dagger_{\nu'} a_{\nu} - a_{\nu}\sum_{\nu\nu'} \epsilon_{\nu\nu'}a_\nu a^\dagger_{\nu'}\\
    &= \sum_{\nu\nu'} \epsilon_{\nu\nu'} a_{\nu} (1- a_\nu a^{\dagger}_{\nu'})- a_{\nu}\sum_{\nu\nu'} \epsilon_{\nu\nu'}a_\nu a^\dagger_{\nu'}\\
    &= \sum_{\nu\nu'} \epsilon_{\nu\nu'} a_{\nu}
\end{flalign*}
Thus
\begin{flalign*}
    \frac{\partial}{\partial t} a_\nu &= \sum_{\nu\nu'} \epsilon_{\nu\nu'} a_{\nu} 
\end{flalign*}
\begin{flalign}
    a_\nu = e^{-i\epsilon t}
\end{flalign}
The equation of motion of the Green's function is:
\begin{flalign}
    G^R(\nu t,\nu't')=-i\theta(t-t')\langle[]
\end{flalign}
\end{document}