\documentclass{article}
\usepackage[fleqn]{amsmath}
\usepackage{esint}
\usepackage{physics}
\usepackage{mathrsfs}
\usepackage{amssymb}
\usepackage{microtype}
\newcommand{\RN}[1]{%s
  \textup{\uppercase\expandafter{\romannumeral#1}}%
}
\usepackage{geometry}
\geometry{
 a4paper,
 left=20mm,
 right=20mm,
 top=15mm,
 bottom=20mm
 }
\begin{document}
\title{Matsubara Summary(2) : Equations}
\maketitle
\section*{Equations for summarizing to derive Green functions}
\begin{flalign}
    S(\nu , \tau) = \frac{1}{\beta} \sum_{ik_n} G(\nu , ik_n) e^{ik\tau}
\end{flalign}
\begin{flalign}
    S_2(\nu_1,\nu_2 ,i\omega ,  \tau) = \frac{1}{\beta} \sum_{ik_n} G_0(\nu , ik_n) G_0 {\nu_2, ik_n + i\omega_n} e^{ik\tau}
\end{flalign}
\begin{flalign}
    S^B(\tau) = \frac{1}{\beta} \sum_{i\omega_n} g(i\omega_n) e^{i\omega_n\tau }
\end{flalign}
\begin{flalign}
    n_B(\tau) = \frac{1}{e^{\beta z }-1}
\end{flalign}
\begin{flalign*}
    {Res}_{z=i\omega_n}[n_B(z)] & = \lim_{z \rightarrow i\omega_n}\frac{(z-i\omega_n)}{e^{\beta z}-1} \\
                                & = \lim_{\delta \rightarrow 0}\frac{\delta}{e^{\beta i \omega_n}e^{\beta\delta} -1} \\
                                & = \frac{1}{\beta}
\end{flalign*}
\begin{flalign*}
    \oint dz n_B(z)g(z) & = 2\pi i \mathop{\mathrm{Res}}_{z = i\omega_n}(n_B(z)g_B(i\omega_n)) \\
                        & = \frac{2 \pi i}{\beta} g(i\omega_n)
\end{flalign*}
\begin{flalign}
    S^B = \int_C \frac{dz}{2\pi i} n_B(z)g(z)
\end{flalign}
\begin{flalign}
    S_0^F(\tau) = \frac{1}{\beta} \sum_{ik_n} g_0(ik_n) e^{ik_n \tau} , \qquad \tau > 0
\end{flalign}
\begin{flalign}
    g_0(z) = \prod_j \frac{1}{z-z_j}
\end{flalign}
\begin{flalign}
    n_F(z)e^{\tau z} = \frac{e^{\tau z}}{e^{\beta z}+1} \propto 
\end{flalign}
\begin{flalign*}
    0 &= \int_{C_\infty} \frac{dz}{2\pi i } n_B(z) g_0(z)e^{\tau z} \\ 
      &= -\frac{1}{\beta} \sum_{ik_n} g_0(ik_n)e^{ik_n\tau} + \sum_j \mathop{\mathrm{Res}}_{z = z_j}(g_0(z))n_F(z_j)e^{\tau_j\tau}
\end{flalign*}
\begin{flalign}
    \frac{1}{\beta} \sum_{i\omega_n}e^{o\omega_n \tau} = S^B_0(\tau) = -\sum_j\mathop{\mathrm{Res}}_{z = z_j}[g_0(z)]n_B(z_j)e^{\tau_j \tau}
\end{flalign}
\begin{flalign}
    S(\tau) = \frac{1}{\beta} \sum_{ik_n}g(ik_n)e^{ik_n\tau}
\end{flalign}
\begin{flalign*}
    S(\tau) &= -\int_{C_1 + C_2} \frac{dz}{2\pi} n_F(z)g(z) e^{z\tau} \\
            &= -\frac{1}{2\pi}\int^\infty_\infty d\epsilon n_F(\epsilon) [g(\epsilon + i\eta)-g(\epsilon -i \eta)]e^{\epsilon\tau}
\end{flalign*}
\begin{flalign}
    \langle a_\nu^\dagger a_\nu\rangle = G(\nu,0^-)
\end{flalign}
\begin{flalign*}
    \leftrightarrow & = \frac{1}{\beta} \sum_{ik_n} G(\nu,ik_n)e^{-ik_n0^-}\\
                    & = G_1(\nu,0^+) \\
                    & = \int^\infty_{-\infty}\frac{d\epsilon}{2\pi} n_F(\epsilon)A(\nu,\epsilon)
\end{flalign*}

 \end{document}