\documentclass{article}
\usepackage[fleqn]{amsmath}
\usepackage{physics}
\usepackage{mathrsfs}
\usepackage{amssymb}
\usepackage{microtype}
\newcommand{\RN}[1]{%s
  \textup{\uppercase\expandafter{\romannumeral#1}}%
}
\usepackage{geometry}
\geometry{
 a4paper,
 left=20mm,
 right=20mm,
 top=15mm,
 bottom=20mm
 }
\begin{document}
\begin{flalign*}
    G^R(\textbf{r}t,\textbf{r}'t')=-i\theta(t-t')\langle[\Psi(\textbf{r}t),\Psi^\dagger(\textbf{r}'t')_{B,F}]\rangle
\end{flalign*}
\begin{flalign*}
    i\frac{\partial}{\partial t}G^R(\textbf{r}t,\textbf{r}'t') &=(-i)(i\partial_t\theta(t-t'))\langle[\Psi(\textbf{r}t),\Psi^\dagger(\textbf{r}'t')_{B,F}]\rangle
    +(-i)\theta(t-t')\langle[i\partial\Psi(\textbf{r}t),\Psi^\dagger(\textbf{r}'t')_{B,F}]\rangle\\
    &=\nabla(t-t')\nabla(\textbf{r}-\textbf{r}')+(-i)\theta(t-t')\langle[i\partial\Psi(\textbf{r}t),\Psi^\dagger(\textbf{r}'t')_{B,F}]\rangle
\end{flalign*}
\begin{flalign*}
    i\partial_t\Psi(\textbf{r}t)=-[H,\Psi(\textbf{r})](t) = -[H_0,\Psi(\textbf{r})](t)-[V_{int},\Psi(\textbf{r})](t)
\end{flalign*}
\begin{flalign*}
    -[H_0,\Psi(r)]&=\frac{1}{2m}\int d\textbf{r}' [\Psi^\dagger(\textbf{r}')\nabla^2_{\textbf{r}'}\Psi^\dagger(\textbf{r}'),\Psi(\textbf{r})]\\
        &= \frac{1}{2m} \nabla^2_{\textbf{r}}\Psi(\textbf{r})
\end{flalign*}
\begin{flalign*}
    \bigg(i\partial_t + \frac{1}{2m}\nabla^2_{\textbf{r}}\bigg)&G^R(\textbf{r}t,\textbf{r}'t')=\nabla(t-t')\nabla(\textbf{r}-\textbf{r}') + D^R(\textbf{r}t,\textbf{r}'t'),
    & D^R(\textbf{r}t,\textbf{r}'t')=-i\theta(t-t')\langle[-V_{int},\psi(\textbf{r})(t),\psi^\dagger(\textbf{r}'t')]_{B,F}\rangle
\end{flalign*}
\begin{flalign*}
    H_0=\sum_{\nu\nu'}t_{\nu'\nu}a^\dagger_{\nu'}a_{\nu'}
\end{flalign*}
\begin{flalign*}
    G^R(\nu t,\nu't')=-i\theta(t-t')\langle[a_{\nu}(t)a_{\nu'}^\dagger(t')]_{B,F}\rangle
\end{flalign*}
\begin{flalign*}
    -[H_0,a_{\nu}]=\sum_{\nu"}t_{\nu\nu"}a_{\nu"}
\end{flalign*}
\begin{flalign*}
    \sum_{\nu"}(i\delta_{\nu\nu"}\partial_t-t_{\nu\nu"})&G^R(\nu"t,\nu't')=\delta(t-t')\delta_{\nu\nu'}+D^R(\nu t,\nu't')\\
     &D^R(\nu t,\nu't')=-i\theta(t-t')\langle\big[-[V_{int},a_\nu](t),a_nu^\dagger]_{B,F}\rangle
\end{flalign*}
\begin{flalign*}
    \sum_{\nu"}[\delta_{\nu\nu"}(\omega + i\eta)-t_{\nu\nu"}]G^R(\nu"\nu';\omega)=\delta_{\nu\nu'}+D^R(\nu\nu';\omega)\\
    D^R(\nu,\nu';\omega)=-i\int^\infty_{-\infty}dt e^{i(\omega+i\eta)(t-t')}\theta(t-t')\langle\bigg[-[V_{int},a_\nu](t),a^\dagger_{\nu'}(t')]_{B,F}\rangle
\end{flalign*}
\begin{flalign*}
    \sum_{\nu"}[\delta_{\nu\nu"}(\omega + i\eta)-t_{\nu\nu"}]G^R(\nu"\nu';\omega)=\delta_{\nu\nu'}
\end{flalign*}
\begin{flalign*}
    (G_0^R)^{-1}(\nu\nu';\omega)=\delta_{\nu\nu'}(\omega+i\eta)-t_{\nu\nu'}\equiv(\textbf{G}_0^R)^{-1}_{\nu\nu'}
\end{flalign*}
\begin{flalign*}
    (\textbf{G}^R_0)^{-1}(\textbf{G}^R_0)=\textbf{1}
\end{flalign*}
\begin{flalign*}
    (\textbf{G}^R_0)_{\nu\nu'}=G^R_0(\nu,\omega)\delta_{\nu\nu'}=\frac{1}{\omega-\epsilon_\nu+i\eta}\delta_{\nu\nu'}
\end{flalign*}
\begin{flalign*}
    H=H_0+H_{hyb} + H_l
\end{flalign*}
\begin{flalign*}
    H_0=\sum_\nu\xi_\nu c_\nu^\dagger c_\nu
\end{flalign*}
\begin{flalign*}
    H_l = \xi_0c_l^\dagger c_l
\end{flalign*}
\begin{flalign*}
    H_{hyb}=\sum_{\nu}(t*_\nu c_\nu^\dagger c_l + t_\nu c_l^\dagger c_\nu)
\end{flalign*}
\begin{flalign*}
    G^R(l,l,t-t')&=-i\theta(t-t')\langle\{c_l(t),c_l^\dagger(t')\}\rangle\\
    G^R(\nu,l,t-t')&=-i\theta(t-t')\langle1\{c_\nu(t),c_.^\dagger(t')\}\rangle
\end{flalign*}
\begin{flalign*}
    (\omega+i\eta-\xi_0)G^R(l,l,\omega)-\sum_\nu t_\nu G^R(\nu,l,\omega)=1\\
    (\omega+i\eta-\xi_\nu)G^R(\nu,l,\omega)-t^*_\nu G^R(l,l,\omega)=0
\end{flalign*}
\begin{flalign}
    H=H+V_{int}
\end{flalign}
\begin{flalign}
    G^R(l,l,\omega)=\frac{1}{\omega-\xi_0-\Sigma^R(\omega)}
\end{flalign}
\begin{flalign}
    \Sigma^R(\omega)=\sum_\nu\frac{|t_\nu|^2}{\omega-\xi_\nu+i\eta}
\end{flalign}
\end{document}