\documentclass{article}
\usepackage{amsmath}
\usepackage{physics}
\usepackage{mathrsfs}
\usepackage{amssymb}
\usepackage{microtype}
\begin{document}
\section*{APPLICATION TO COUPLED CAVITY ARRAY}
\subsection*{Bound states, symmetry-protected BIC, quasi-BIC}
\begin{equation*}
    \hat{H}_light = -\frac{J}{2} \sum_{x} (\hat{a}^\dagger_{x+1}\hat{a}_x + H.c.) + \hbar\omega_c \sum_{x} \hat{a}_x^\dagger \hat{a}_x
\end{equation*}
$\omega_c$ \\ $\hat{a}_x \equiv \frac{1}{\sqrt{L}} \sum_k \hat{a}_k e^{-ikx}$
\begin{equation*}
    \hbar\omega_k = \hbar\omega_c - J cos k
\end{equation*}
\begin{equation*}
    \hat{A}=\textit{A}(\hat{a}_{x=0} + \hat{a}_{x=0}^\dagger)
\end{equation*}
$\textit{f}_k=\frac{\textit{A}}{\sqrt{L}}$ \\
$g=q\textit{A}\sqrt{\frac{\omega_c}{m\hbar}}$\\
$V(Q) = v\big( 1-\frac{Q^2}{d^2}\big)^2$ \\
$\Omega_0$
$\frac{(E_2 - E_1)}{\hbar} \simeq \omega_c $\\
\begin{equation*}
    \delta E_{sca} \in [\hbar\omega_c - J , \hbar\omega_c + J]
\end{equation*}
\begin{equation*}
    \delta E_{BS} \notin [\hbar\omega_c - J , \hbar\omega_c + J]
\end{equation*}
\begin{equation*}
    \delta E_{(q)BIC} \in [\hbar\omega_c - J , \hbar\omega_c + J]
\end{equation*}
\begin{equation*}
    \Gamma_{qBIC} ~ \frac{(J/\hbar)^2}{g\sqrt{m\omega_c^3d^3}}\bigg(\frac{v^3}{m_{eff}}\bigg)^{1/4}
    \propto g^{-3/2}
\end{equation*}
\subsection*{Dressed potential}
\begin{equation*}
    V_{eff}(Q) = v_{eff}\bigg(1-\frac{Q^2}{d_{eff}}\bigg)^2
\end{equation*}
\begin{equation*}
    v_{eff}=\begin{cases}
        v\big(1-\frac{3\xi^2}{d^2}\big)^2, & \xi \leq \frac{d}{\sqrt{3}},\\
        0, & \frac{d}{\sqrt{3}}
    \end{cases}
\end{equation*}
\subsection*{Two-level effective model and its breakdown in the Coulomb gauge}
\begin{equation*}
    \hat{H}^{JC}_{U} = \frac{\hbar \Delta_g}{2}\hat{\sigma}^z + \bigg(\hat{\sigma}^- \sum_n \hbar\tilde{g}_n\hat{b}_n^{\dagger} + H.c.\bigg)
    + \sum_n \hbar\Omega_n \hat{b}_n^\dagger \hat{b}_n
\end{equation*}
\begin{equation*}
    \Delta_g \equiv \frac{E_2 - E_1}{\hbar} > 0,
\end{equation*}
\begin{equation*}
    \tilde{g}_n \frac{\xi}{\hbar}\bra{\psi_1}\frac{dV}{dQ}\ket{\psi_2}
\end{equation*}
\begin{equation*}
    E_{ex} - \Delta_g = \sum_n \frac{\tilde{g}^2_n}{E_{ex} - \Omega_n}
\end{equation*}
\begin{equation*}
    \hat{H}^{JC}_{U} = \frac{\hbar \Delta}{2}\hat{\sigma}^z + \bigg(\hat{\sigma}^- \sum_k \hbar\tilde{g}_k\hat{a}_k^{\dagger} + H.c.\bigg)
    + \sum_k \hbar\Omega_k \hat{a}_k^\dagger \hat{a}_k
\end{equation*}
$\Delta \equiv \Delta_{g=0}$
\begin{equation*}
    \tilde{g}_k \equiv \frac{g}{\sqrt{L}} \kappa_{\omega_c}\bra{\psi_1^{g=0}}\partial_Q\ket{\psi_2^{g=0}}
\end{equation*} 
\begin{equation*}
    \hat{H}^{Rabi}_{U} = \frac{\hbar \Delta_g}{2}\hat{\sigma}^z + \hat{\sigma}^x \bigg( \sum_n \hbar\tilde{g}_n\hat{b}_n^{\dagger} + H.c.\bigg)
    + \sum_n \hbar\Omega_n \hat{b}_n^\dagger \hat{b}_n
\end{equation*}
\begin{equation*}
    \ket{\Psi(t)}_U = e^{-i\hat{H}_U t}\ket{\Psi(0)}_U = \sum_i c_i e^{-iE_it} \ket{\Psi_i}_U
\end{equation*}
\begin{equation*}
    \langle \hat{O} \rangle_C = \langle \hat{U}^\dagger \hat{O} \hat{U} \rangle _U
\end{equation*}
\begin{equation*}
    \omega_{osc} = \sqrt{\frac{8v}{d^2_f m_{eff}}\bigg(1-\frac{3\xi^2}{d^2_f}\bigg)} \propto g^{-1}
\end{equation*}
    \end{document}