\documentclass[9pt]{article}
\usepackage{amsmath}
\usepackage{physics}
\usepackage{mathrsfs}
\usepackage{amssymb}
\usepackage{microtype}
\begin{document}
\begin{equation*}
    \Delta X_1 = \frac{1}{2}e^{-r}, \Delta X_2 = \frac{1}{2}e^{-r}
\end{equation*}
\begin{equation*}
    \hat{X_1} \rightarrow \hat{X_1} e^{-r} , \hat{X_2} \rightarrow \hat{X_2} e^{-r}
\end{equation*}
\begin{equation*}
    (\hat{a}+\hat{a}^{\dagger}) \rightarrow (\hat{a}+\hat{a}^{\dagger})e^{-r} , (\hat{a}-\hat{a}^{\dagger}) \rightarrow (\hat{a}-\hat{a}^{\dagger})e^{-r}
\end{equation*}
\begin{equation*}
    \hat{a} \rightarrow \hat{b} = \hat{a} \hypcosine{r} - \hat{a}^{\dagger} \hypsine{r}
\end{equation*}
\begin{equation*}
    \hat{a} \rightarrow \hat{b}^{\dagger} = \hat{a}^{\dagger} \hypcosine{r} - \hat{a}^{\dagger} \hypsine{r}
\end{equation*}
If Operator $ \hat{S}(r) $ is,
\begin{equation*}
    \hat{S}^{\dagger} (r) \hat{a} \hat{S}(r) = \hat{b} = \hat{a} \hypcosine{r} - \hat{a}^{\dagger} \hypsine{r}
\end{equation*}
\begin{equation*}
    \hat{S}^{\dagger} (r) \hat{a}^{\dagger} \hat{S}(r) = \hat{b} = \hat{a}^{\dagger} \hypcosine{r} - \hat{a} \hypsine{r}
\end{equation*}
Or,
\begin{equation*}
    \hat{S}^{\dagger} (r) \hat{X_1} \hat{S}(r) = \hat{X_1}e^{-r}
\end{equation*}
\begin{equation*}
    \hat{S}^{\dagger} (r) \hat{X_2} \hat{S}(r) = \hat{X_2}e^{r}
\end{equation*}
Then Squeezed state given by:
\begin{equation*}
    \ket{r,\alpha}=\hat{S}(r)\ket{\alpha}=\hat{S}(r)\hat{D}(\alpha)\ket{0}
\end{equation*}
The Operator which satisfies the above equation is given by:
\begin{equation*}
    \hat{S}(r)=e^{\frac{r}{2}\hat{a}^2-\frac{r}{2}\hat{a}^{\dagger 2}}
\end{equation*}
For any complex number $ z=re^{i\theta} $,
\begin{equation*}
    \hat{S}(r)=e^{\frac{z^*}{2}\hat{a}^2-\frac{z}{2}\hat{a}^{\dagger 2}}
\end{equation*}

Optimize  $\abs{F(x,y)-G(x,y,z)}$  where  $F=4x+y$ , $G=0.875(x+y+z)$

\end{document}